src/Ext/ExprDI.v
@@ -13,21 +13,22 @@ Set Strict Implicit.
 
 Module Type ExprDenote_core.
 
-  Parameter exprD' : forall (ts : types) (fs : functions ts),
-    env (typD ts) -> forall g : list typ, expr -> forall t : typ,
+  Parameter exprD' : forall {ts : types} {func : Type} {_ : RFunc (typD ts) func},
+    env (typD ts) -> forall g : list typ, expr func -> forall t : typ,
     option (hlist (typD ts nil) g -> typD ts nil t).
 
   Section with_envs.
     Variable ts : types.
-    Variable fs : functions ts.
+    Variable func : Type.
+    Variable RFunc_func : RFunc (typD ts) func.
     Variable us : env (typD ts).
 
     Axiom exprD'_Abs : forall ve t e u,
-       exprD' fs us ve (Abs t e) u =
+       exprD' us ve (Abs t e) u =
        match u as u return option (hlist (typD ts nil) ve -> typD ts nil u) with
          | tvArr l r =>
            match typ_cast_typ _ (fun x => x) _ l t
-               , exprD' fs us (t :: ve) e r
+               , exprD' us (t :: ve) e r
            with
              | Some cast , Some f =>
                Some (fun g => fun x => f (Hcons (F := typD ts nil) (cast x) g))
@@ -37,7 +38,7 @@ Module Type ExprDenote_core.
        end.
 
     Axiom exprD'_Var : forall ve v t,
-      exprD' fs us ve (Var v) t =
+      exprD' us ve (Var v) t =
       match nth_error ve v as z
             return z = nth_error ve v ->
                    option (hlist (typD ts nil) ve -> typD ts nil t)
@@ -58,55 +59,25 @@ Module Type ExprDenote_core.
       end eq_refl.
 
     Axiom exprD'_UVar : forall ve u t,
-      exprD' fs us ve (UVar u) t =
+      exprD' us ve (UVar u) t =
       match lookupAs us u t with
         | Some z => Some (fun _ => z)
         | None => None
       end.
 
-    Axiom exprD'_Func : forall ve f ts t,
-      exprD' fs us ve (Func f ts) t =
-      match nth_error fs f with
+    Axiom exprD'_Func : forall ve f t,
+      exprD' us ve (Inj f) t =
+      match funcAs f t with
         | None => None
-        | Some f =>
-          match type_apply _ _ ts _ _ f.(fdenote) with
-            | None => None
-            | Some t' =>
-              match @typ_cast_typ _ (fun x => x) _ (instantiate_typ ts (ftype f)) t with
-                | None => None
-                | Some cast => Some (fun _ => cast t')
-              end
-          end
-      end.
-
-    Axiom exprD'_Equal : forall ve t l r t',
-      exprD' fs us ve (Equal t l r) t' =
-      match t' as t' return option (hlist (typD ts nil) ve -> typD ts nil t') with
-        | tvProp =>
-          match exprD' fs us ve l t , exprD' fs us ve r t with
-            | Some l , Some r => Some (fun g => l g = r g)
-            | _ , _ => None
-          end
-        | _ => None
-      end.
-
-    Axiom exprD'_Not : forall ve p t',
-      exprD' fs us ve (Not p) t' =
-      match t' as t' return option (hlist (typD ts nil) ve -> typD ts nil t') with
-        | tvProp =>
-          match exprD' fs us ve p tvProp with
-            | Some p => Some (fun g => not (p g))
-            | _ => None
-          end
-        | _ => None
+        | Some val => Some (fun _ => val)
       end.
 
     Axiom exprD'_App : forall ve t e arg,
-      exprD' fs us ve (App e arg) t =
-      match typeof_expr (typeof_funcs fs) (typeof_env us) ve e with
+      exprD' us ve (App e arg) t =
+      match typeof_expr (typeof_env us) ve e with
         | Some (tvArr l r) =>
-          match exprD' fs us ve e (tvArr l r)
-              , exprD' fs us ve arg l
+          match exprD' us ve e (tvArr l r)
+              , exprD' us ve arg l
               , typ_cast_typ _ (fun x => x) _ r t
           with
             | Some f , Some x , Some cast =>
@@ -134,92 +105,58 @@ Module Type ExprDenote.
    ** there is an error before needing to get the variables.
    **
    **)
-  Definition exprD ts fs us vs e t : option (typD ts nil t) :=
+  Definition exprD {ts} {func : Type} {fs : RFunc (typD ts) func} us vs e t
+  : option (typD ts nil t) :=
     let (tvs,gvs) := split_env vs in
-    match @exprD' ts fs us tvs e t with
+    match @exprD' ts func fs us tvs e t with
       | None => None
       | Some f => Some (f gvs)
     end.
 
   Section with_envs.
     Variable ts : types.
-    Variable fs : functions ts.
+    Variable func : Type.
+    Variable RFunc_func : RFunc (typD ts) func.
     Variable us : env (typD ts).
 
     Axiom typeof_exprD : forall vs e t,
-      typeof_expr (typeof_funcs fs) (typeof_env us) vs e = Some t ->
-      exists val, exprD' fs us vs e t = Some val.
+      typeof_expr (typeof_env us) vs e = Some t ->
+      exists val, exprD' us vs e t = Some val.
 
     Axiom exprD_Var : forall ve v t,
-      exprD fs us ve (Var v) t = lookupAs ve v t.
+      exprD us ve (Var v) t = lookupAs ve v t.
 
     Axiom exprD_UVar : forall ve u t,
-      exprD fs us ve (UVar u) t = lookupAs us u t.
+      exprD us ve (UVar u) t = lookupAs us u t.
 
-    Axiom exprD_Func : forall ve f ts t,
-      exprD fs us ve (Func f ts) t =
-      match nth_error fs f with
-        | None => None
-        | Some f =>
-          match type_apply _ _ ts _ _ f.(fdenote) with
-            | None => None
-            | Some t' =>
-              @typ_cast_val _ _ (instantiate_typ ts (ftype f)) t t'
-          end
-      end.
-
-    Axiom exprD_Equal : forall ve t l r t',
-      exprD fs us ve (Equal t l r) t' =
-      match t' as t' return option (typD ts nil t') with
-        | tvProp =>
-          match exprD fs us ve l t , exprD fs us ve r t with
-            | Some l , Some r => Some (l = r)
-            | _ , _ => None
-          end
-        | _ => None
-      end.
-
-    Axiom exprD_Not : forall ve p t',
-      exprD fs us ve (Not p) t' =
-      match t' as t' return option (typD ts nil t') with
-        | tvProp =>
-          match exprD fs us ve p tvProp with
-            | Some p => Some (~p)
-            | _ => None
-          end
-        | _ => None
-      end.
+    Axiom exprD_Func : forall ve f t,
+      exprD us ve (Inj f) t = funcAs f t.
 
     Axiom exprD_Abs_is_arr : forall vs e t t',
-      exprD fs us vs (Abs t' e) t =
+      exprD us vs (Abs t' e) t =
       match t as t return option (typD ts nil t) with
         | tvArr l r =>
           if t' ?[ eq ] l then
-            exprD fs us vs (Abs l e) (tvArr l r)
+            exprD us vs (Abs l e) (tvArr l r)
           else None
         | _ => None
       end.
 
     Axiom typeof_expr_eq_exprD_False : forall l ve e t,
-      WellTyped_expr (typeof_funcs fs) (typeof_env us) (l :: typeof_env ve) e t ->
-      forall x, exprD fs us (existT _ l x :: ve) e t = None ->
+      WellTyped_expr (typeof_env us) (l :: typeof_env ve) e t ->
+      forall x, exprD us (existT _ l x :: ve) e t = None ->
                 False.
 
     Axiom typeof_expr_exprD' : forall vs e t,
-      WellTyped_expr (typeof_funcs fs) (typeof_env us) vs e t <->
-      exists v, exprD' fs us vs e t = Some v.
-(*
-    Axiom exprD_Abs : forall ve t u e val,
-      exprD fs us ve (Abs t e) (tvArr t u) = Some val ->
-      forall x, exprD fs us (existT _ t x :: ve) e u = Some (val x).
-*)
+      WellTyped_expr (typeof_env us) vs e t <->
+      exists v, exprD' us vs e t = Some v.
 
     Axiom exprD_App : forall ve t e arg,
-      exprD fs us ve (App e arg) t =
-      match typeof_expr (typeof_funcs fs) (typeof_env us) (typeof_env ve) e with
+      exprD us ve (App e arg) t =
+      match typeof_expr (typeof_env us) (typeof_env ve) e with
         | Some (tvArr l r) =>
-          match exprD fs us ve e (tvArr l r)
-              , exprD fs us ve arg l
+          match exprD us ve e (tvArr l r)
+              , exprD us ve arg l
               , typ_cast_typ _ (fun x => x) _ r t
           with
             | Some f , Some x , Some cast =>
@@ -233,31 +170,31 @@ Module Type ExprDenote.
 
 End ExprDenote.
 
-
-
 Module Build_ExprDenote (EDc : ExprDenote_core) <:
-       ExprDenote with Definition exprD' := EDc.exprD'.
+       ExprDenote with Definition exprD' := @EDc.exprD'.
   Require Import ExtLib.Tactics.Consider.
   Require Import ExtLib.Tactics.Injection.
   Require Import ExtLib.Data.ListNth.
 
   Include EDc.
 
-  Definition exprD ts fs us vs e t : option (typD ts nil t) :=
+  Definition exprD {ts} {func} {fs : RFunc (typD ts) func} us vs e t
+  : option (typD ts nil t) :=
     let (tvs,gvs) := split_env vs in
-    match @exprD' ts fs us tvs e t with
+    match @exprD' ts _ fs us tvs e t with
       | None => None
       | Some f => Some (f gvs)
     end.
 
   Section with_envs.
     Variable ts : types.
-    Variable fs : functions ts.
+    Variable func : Type.
+    Variable RFunc_func : RFunc (typD ts) func.
     Variable us : env (typD ts).
 
     Theorem typeof_exprD : forall vs e t,
-      typeof_expr (typeof_funcs fs) (typeof_env us) vs e = Some t ->
-      exists val, exprD' fs us vs e t = Some val.
+      typeof_expr (typeof_env us) vs e = Some t ->
+      exists val, exprD' us vs e t = Some val.
     Proof.
       intros vs e; revert vs.
       induction e; simpl; intros.
@@ -271,14 +208,9 @@ Module Build_ExprDenote (EDc : ExprDenote_core) <:
         intros. subst.
         rewrite typ_cast_typ_refl. eauto. }
       { rewrite exprD'_Func.
-        unfold typeof_funcs in *.
-        rewrite nth_error_map in H.
-        destruct (nth_error fs f); try congruence.
-        change EqNat.beq_nat with (@rel_dec _ (@eq nat) _) in H.
-        consider (length l ?[ eq ] tfenv (typeof_func f0)); intros; try congruence.
-        eapply type_apply_length_equal in H. destruct H. rewrite H.
-        inv_all; subst.
-        destruct f0; simpl in *.
+        unfold funcAs.
+        generalize (funcD f). rewrite H. intros.
+        simpl.
         rewrite typ_cast_typ_refl. eauto. }
       { rewrite exprD'_App.
         specialize (IHe1 vs). specialize (IHe2 vs).
@@ -296,7 +228,7 @@ Module Build_ExprDenote (EDc : ExprDenote_core) <:
         eauto. }
       { rewrite exprD'_Abs.
         specialize (IHe (t :: vs)).
-        destruct (typeof_expr (typeof_funcs fs) (typeof_env us) (t :: vs) e); try congruence.
+        destruct (typeof_expr (typeof_env us) (t :: vs) e); try congruence.
         inv_all; subst.
         specialize (IHe _ eq_refl).
         destruct IHe.
@@ -307,27 +239,10 @@ Module Build_ExprDenote (EDc : ExprDenote_core) <:
         destruct (nth_error us u); try congruence.
         inv_all; subst. destruct s; simpl.
         rewrite typ_cast_typ_refl. eauto. }
-      { rewrite exprD'_Equal.
-        specialize (IHe1 vs). specialize (IHe2 vs).
-        change typ_eqb with (@rel_dec _ (@eq typ) _) in *.
-        repeat match goal with
-                 | _ : match ?X with _ => _ end = _ |- _ =>
-                   consider X; intros; try congruence
-               end.
-        destruct (IHe1 _ eq_refl); destruct (IHe2 _ eq_refl).
-        inv_all; subst. subst.
-        rewrite H5. rewrite H4. eauto. }
-      { specialize (IHe vs).
-        rewrite exprD'_Not.
-        destruct (typeof_expr (typeof_funcs fs) (typeof_env us) vs e); try congruence.
-        destruct t0; try congruence.
-        inv_all; subst.
-        destruct (IHe _ eq_refl). rewrite H.
-        eauto. }
     Qed.
 
     Theorem exprD_Var : forall ve u t,
-      exprD fs us ve (Var u) t = lookupAs ve u t.
+      exprD us ve (Var u) t = lookupAs ve u t.
     Proof.
       unfold exprD; intros.
       consider (split_env ve); intros.
@@ -452,7 +367,7 @@ Module Build_ExprDenote (EDc : ExprDenote_core) <:
     Qed.
 
     Theorem exprD_UVar : forall ve u t,
-      exprD fs us ve (UVar u) t = lookupAs us u t.
+      exprD us ve (UVar u) t = lookupAs us u t.
     Proof.
       unfold exprD; intros.
       destruct (split_env ve).
@@ -463,71 +378,21 @@ Module Build_ExprDenote (EDc : ExprDenote_core) <:
       destruct (TypesI.typ_cast (fun x1 : Type => x1) nil x0 t); auto.
     Qed.
 
-    Theorem exprD_Func : forall ve f ts t,
-      exprD fs us ve (Func f ts) t =
-      match nth_error fs f with
-        | None => None
-        | Some f =>
-          match type_apply _ _ ts _ _ f.(fdenote) with
-            | None => None
-            | Some t' =>
-              @typ_cast_val _ _ (instantiate_typ ts (ftype f)) t t'
-          end
-      end.
+    Theorem exprD_Func : forall ve f t,
+      exprD us ve (Inj f) t = funcAs f t.
     Proof.
       unfold exprD. intros.
       destruct (split_env ve).
       rewrite exprD'_Func.
-      destruct (nth_error fs f); auto.
-      destruct (type_apply ts (fenv f0) ts0 nil (ftype f0) (fdenote f0)); auto.
-      unfold typ_cast_val.
-      destruct (typ_cast_typ ts (fun x0 : Type => x0) nil
-       (instantiate_typ ts0 (ftype f0)) t); auto.
-    Qed.
-
-    Theorem exprD_Equal : forall ve t l r t',
-      exprD fs us ve (Equal t l r) t' =
-      match t' as t' return option (typD ts nil t') with
-        | tvProp =>
-          match exprD fs us ve l t , exprD fs us ve r t with
-            | Some l , Some r => Some (l = r)
-            | _ , _ => None
-          end
-        | _ => None
-      end.
-    Proof.
-      unfold exprD. intros.
-      destruct (split_env ve).
-      rewrite exprD'_Equal.
-      destruct t'; auto.
-      destruct (exprD' fs us x l t); auto.
-      destruct (exprD' fs us x r t); auto.
-    Qed.
-
-    Theorem exprD_Not : forall ve p t',
-      exprD fs us ve (Not p) t' =
-      match t' as t' return option (typD ts nil t') with
-        | tvProp =>
-          match exprD fs us ve p tvProp with
-            | Some p => Some (~p)
-            | _ => None
-          end
-        | _ => None
-      end.
-    Proof.
-      unfold exprD; intros.
-      destruct (split_env ve).
-      rewrite exprD'_Not.
-      destruct t'; auto.
-      destruct (exprD' fs us x p tvProp); auto.
+      destruct (funcAs f t); auto.
     Qed.
 
     Theorem exprD_App : forall ve t e arg,
-      exprD fs us ve (App e arg) t =
-      match typeof_expr (typeof_funcs fs) (typeof_env us) (typeof_env ve) e with
+      exprD us ve (App e arg) t =
+      match typeof_expr (typeof_env us) (typeof_env ve) e with
         | Some (tvArr l r) =>
-          match exprD fs us ve e (tvArr l r)
-              , exprD fs us ve arg l
+          match exprD us ve e (tvArr l r)
+              , exprD us ve arg l
               , typ_cast_typ _ (fun x => x) _ r t
           with
             | Some f , Some x , Some cast =>
@@ -542,19 +407,22 @@ Module Build_ExprDenote (EDc : ExprDenote_core) <:
       destruct (split_env ve).
       rewrite exprD'_App.
       simpl in *. unfold typeof_env.
-      destruct (typeof_expr (typeof_funcs fs) (map (projT1 (P:=typD ts nil)) us) x e); auto.
+      destruct (typeof_expr (map (projT1 (P:=typD ts nil)) us) x e); auto.
       destruct t0; auto.
-      destruct (exprD' fs us x e (tvArr t0_1 t0_2)); auto.
-      destruct (exprD' fs us x arg t0_1); auto.
+      repeat match goal with
+               | |- match match ?X with _ => _ end with _ => _ end =
+                    match match ?Y with _ => _ end with _ => _ end =>
+                 change X with Y; destruct Y; auto
+             end.
       destruct (typ_cast_typ ts (fun x0 : Type => x0) nil t0_2 t); auto.
     Qed.
 
     Theorem exprD_Abs_is_arr : forall vs e t t',
-      exprD fs us vs (Abs t' e) t =
+      exprD us vs (Abs t' e) t =
       match t as t return option (typD ts nil t) with
         | tvArr l r =>
           if t' ?[ eq ] l then
-            exprD fs us vs (Abs l e) (tvArr l r)
+            exprD us vs (Abs l e) (tvArr l r)
           else None
         | _ => None
       end.
@@ -573,21 +441,26 @@ Module Build_ExprDenote (EDc : ExprDenote_core) <:
     Qed.
 
     Theorem typeof_expr_eq_exprD_False : forall l ve e t,
-      WellTyped_expr (typeof_funcs fs) (typeof_env us) (l :: typeof_env ve) e t ->
-      forall x, exprD fs us (existT _ l x :: ve) e t = None ->
+      WellTyped_expr (typeof_env us) (l :: typeof_env ve) e t ->
+      forall x, exprD us (existT _ l x :: ve) e t = None ->
                 False.
     Proof.
       intros. unfold exprD in *. simpl in *.
-      consider (exprD' fs us (l :: projT1 (split_env ve)) e t); try congruence; intros.
       unfold WellTyped_expr in *.
       eapply typeof_exprD in H. destruct H.
-      rewrite split_env_projT1 in H0. unfold typeof_env in *.
-      congruence.
+      revert H0 H.
+      generalize (projT2 (split_env ve)).
+      rewrite split_env_projT1.
+      intros.
+      match goal with
+        | H : ?Y = _ , H' : match ?X with _ => _ end = _ |- _ =>
+          change X with Y in * ; rewrite H in H'
+      end. congruence.
     Qed.
 
     Lemma lem_typeof_expr_exprD' : forall vs e t,
-      WellTyped_expr (typeof_funcs fs) (typeof_env us) vs e t <->
-      exprD' fs us vs e t <> None.
+      WellTyped_expr (typeof_env us) vs e t <->
+      exprD' us vs e t <> None.
     Proof.
       intros vs e. revert vs. induction e; simpl; intros.
       { rewrite WellTyped_expr_Var.
@@ -671,45 +544,31 @@ Module Build_ExprDenote (EDc : ExprDenote_core) <:
           apply (typ_cast_typ_eq _ _ _ _ _ H). } }
       { rewrite WellTyped_expr_Func.
         rewrite exprD'_Func.
-        rewrite nth_error_typeof_funcs.
-        destruct (nth_error fs f).
-        { split; intro.
-          { destruct H; intuition try congruence.
-            inv_all. subst.
-            destruct f0; simpl in *.
-            destruct (type_apply_length_equal _ _ _ _ fdenote H).
-            rewrite H1 in *.
-            rewrite typ_cast_typ_refl in H0. congruence. }
-          { eexists. split; eauto.
-            repeat match goal with
-                     | _ : not (match ?X with _ => _ end = _) |- _ =>
-                       consider X; intros
-                   end; try congruence.
-            eapply type_apply_length_equal' in H.
-            destruct f0; simpl in *; split; auto.
-            generalize (typ_cast_typ_eq _ _ _ _ _ H0); auto. } }
-        { split; intros.
-          { destruct H; intuition; congruence. }
-          { congruence. } } }
+        unfold funcAs.
+        generalize (funcD f).
+        destruct (typeof_func f); intuition; try congruence.
+        { inv_all; subst. simpl in *.
+          rewrite typ_cast_typ_refl in *. congruence. }
+        { simpl in *. admit. } }
       { rewrite WellTyped_expr_App.
         rewrite exprD'_App.
         split; intros.
         { destruct H. destruct H.
           rewrite IHe1 in *. rewrite IHe2 in *.
           destruct H. destruct H0.
-          consider (typeof_expr (typeof_funcs fs) (typeof_env us) vs e1); intros.
+          consider (typeof_expr (typeof_env us) vs e1); intros.
           { generalize H. generalize H0.
             eapply IHe1 in H. eapply IHe2 in H0.
             red in H; red in H0. rewrite H in H2. inv_all; subst.
             destruct t0; simpl in *; try congruence.
             change typ_eqb with (@rel_dec _ (@eq typ) _) in *.
             consider (t0_1 ?[ eq ] x0); try congruence; intros; inv_all; subst.
-            destruct (exprD' fs us vs e1 (tvArr x0 t)); intuition.
-            destruct (exprD' fs us vs e2 x0); intuition.
+            destruct (exprD' us vs e1 (tvArr x0 t)); intuition.
+            destruct (exprD' us vs e2 x0); intuition.
             rewrite typ_cast_typ_refl in H1; congruence. }
           { exfalso.
             eapply IHe1 in H. red in H. congruence. } }
-        { consider (typeof_expr (typeof_funcs fs) (typeof_env us) vs e1);
+        { consider (typeof_expr (typeof_env us) vs e1);
           try congruence; intros.
           destruct t0; try congruence.
           repeat match goal with
@@ -717,7 +576,7 @@ Module Build_ExprDenote (EDc : ExprDenote_core) <:
                      consider X; intros
                  end; try congruence.
           generalize (typ_cast_typ_eq _ _ _ _ _ H2); intros.
-          consider (exprD' fs us vs e1 (tvArr t0_1 t0_2)); intros; try congruence.
+          consider (exprD' us vs e1 (tvArr t0_1 t0_2)); intros; try congruence.
           inv_all. rewrite H5 in *.
           exists (tvArr t0_1 t0_2). exists t0_1.
           simpl.
@@ -731,7 +590,7 @@ Module Build_ExprDenote (EDc : ExprDenote_core) <:
         { split; intros.
           { destruct H. destruct H; subst.
             rewrite typ_cast_typ_refl.
-            consider (exprD' fs us (t :: vs) e x); try congruence.
+            consider (exprD'  us (t :: vs) e x); try congruence.
             intros. intro. eapply IHe; eauto. }
           { destruct t0; intuition try congruence.
             repeat match goal with
@@ -761,41 +620,16 @@ Module Build_ExprDenote (EDc : ExprDenote_core) <:
             inv_all; subst.
             f_equal; eapply (typ_cast_typ_eq _ _ _ _ _ H). } }
         { intuition congruence. } }
-      { rewrite WellTyped_expr_Equal.
-        rewrite exprD'_Equal.
-        split; intros.
-        { destruct H; subst.
-          rewrite IHe1 in H0. rewrite IHe2 in H0.
-          destruct H0.
-          repeat match goal with
-                   | |- not (match ?X with _ => _ end = _) =>
-                     destruct X; try congruence
-                 end. }
-        { destruct t0; try solve [ intuition ].
-          split; auto.
-          rewrite IHe1. rewrite IHe2.
-          repeat match goal with
-                   | _ : not (match ?X with _ => _ end = _) |- _ =>
-                     destruct X
-                 end; intuition congruence. } }
-      { rewrite WellTyped_expr_Not.
-        rewrite exprD'_Not.
-        split.
-        { destruct t; intuition try congruence.
-          eapply IHe; eauto.
-          destruct (exprD' fs us vs e tvProp); congruence. }
-        { destruct t; intuition.
-          eapply IHe. intros. rewrite H0 in *. intuition. } }
     Qed.
 
     Theorem typeof_expr_exprD' : forall vs e t,
-      WellTyped_expr (typeof_funcs fs) (typeof_env us) vs e t <->
-      exists v, exprD' fs us vs e t = Some v.
+      WellTyped_expr (typeof_env us) vs e t <->
+      exists v, exprD' us vs e t = Some v.
     Proof.
       intros.
       rewrite lem_typeof_expr_exprD'.
       intuition.
-      destruct (exprD' fs us vs e t); intuition. eauto.
+      destruct (exprD' us vs e t); intuition. eauto.
       destruct H. congruence.
     Qed.
 
