src/Ext/ExprD.v
@@ -9,14 +9,14 @@ Set Strict Implicit.
 
 Include EXPR_DENOTE.
 
-Instance Expr_expr ts (fs : functions ts) : Expr (typD ts) expr :=
-{ exprD := exprD fs
-; Safe_expr := WellTyped_expr (typeof_funcs fs)
-; acc := expr_acc
-; wf_acc := wf_expr_acc
+Instance Expr_expr ts func (RFunc_func : RFunc (typD ts) func) : Expr (typD ts) (expr func) :=
+{ exprD := exprD
+; Safe_expr := @WellTyped_expr _ _ RFunc_func
+; acc := @expr_acc _
+; wf_acc := @wf_expr_acc _
 }.
 
 Create HintDb exprD_rw discriminated.
 
-Hint Rewrite exprD_Var exprD_App exprD_UVar exprD_Equal exprD_Not exprD_Func : exprD_rw.
-Hint Rewrite exprD'_Abs exprD'_Var exprD'_App exprD'_UVar exprD'_Equal exprD'_Not exprD'_Func : exprD_rw.
+Hint Rewrite exprD_Var exprD_App exprD_UVar exprD_Func : exprD_rw.
+Hint Rewrite exprD'_Abs exprD'_Var exprD'_App exprD'_UVar exprD'_Func : exprD_rw.
